Clean proofs for comp_out_rel_cases

pancake/proofs/crep_to_loopProofScript.sml
@@ -71,6 +71,30 @@ Termination
   cheat
 End
 
+Definition cut_sets_def:
+  (cut_sets l Skip = l) ∧
+  (cut_sets l (LocValue n m) = insert n () l) ∧
+  (cut_sets l (Assign n e) = insert n () l) ∧
+  (cut_sets l (LoadByte n e m) = insert m () l) ∧
+  (cut_sets l (Seq p q) = cut_sets (cut_sets l p) q) ∧
+  (cut_sets l (If _ _ _ p q nl) = nl) ∧
+  (cut_sets _ _ = ARB)
+End
+
+
+
+Definition comp_syntax_ok_def:
+  comp_syntax_ok l p <=>
+    p = Skip ∨
+    ?n m. p = LocValue n m ∨
+    ?n e. p = Assign n e ∨
+    ?n e m. p = LoadByte n e m ∨
+    ?c n m v v'. p = If c n (Reg m) (Assign n v) (Assign n v') (list_insert [n; m] l) ∨
+    ?q r. p = Seq q r ∧ comp_syntax_ok l q ∧ comp_syntax_ok (cut_sets l q) r
+Termination
+ cheat
+End
+
 Definition compile_prog_def:
   (compile_prog _ l (Skip:'a crepLang$prog) = (Skip:'a loopLang$prog, l)) /\
   (compile_prog ctxt l (Assign v e) =
@@ -178,6 +202,8 @@ Definition locals_rel_def:
     lookup n t_locals = SOME v' ∧ wlab_wloc ctxt v = v'
 End
 
+(* theorems start from here *)
+
 Theorem state_rel_intro:
   state_rel ^s (t:('a,'ffi) loopSem$state) <=>
   s.memaddrs = t.mdomain ∧
@@ -261,95 +287,72 @@ val evaluate_nested_seq_append_first = evaluate_nested_seq_cases |> CONJUNCT1
 val evaluate_none_nested_seq_append = evaluate_nested_seq_cases |> CONJUNCT2 |> CONJUNCT1
 val evaluate_not_none_nested_seq_append = evaluate_nested_seq_cases |> CONJUNCT2 |> CONJUNCT2
 
-Definition comp_syntax_ok_def:
-  comp_syntax_ok p = every_prog
-  (λp. p = Skip ∨
-   ?n m. p = LocValue n m ∨
-   ?n e. p = Assign n e ∨
-   ?n e m. p = LoadByte n e m ∨
-   (?c n m ns v v'. p = If c n (Reg m) (Assign n v) (Assign n v') ns) ∨
-   (?q r. p = Seq q r ∧ comp_syntax_ok q ∧ comp_syntax_ok r)) p
-Termination
- cheat
-End
-
-
 Theorem comp_syn_ok_basic_cases:
-  comp_syntax_ok Skip /\ (!n m. comp_syntax_ok (LocValue n m)) /\
-  (!n e. comp_syntax_ok (Assign n e)) /\  (!n e m. comp_syntax_ok (LoadByte n e m)) /\
-  (!c n m ns v v'. comp_syntax_ok (If c n (Reg m) (Assign n v) (Assign n v') ns))
+  (!l. comp_syntax_ok l Skip) /\ (!l n m. comp_syntax_ok l (LocValue n m)) /\
+  (!l n e. comp_syntax_ok l (Assign n e)) /\  (!l n e m. comp_syntax_ok l (LoadByte n e m)) /\
+  (!l c n m v v'. comp_syntax_ok l (If c n (Reg m) (Assign n v) (Assign n v') (list_insert [n; m] l)))
 Proof
   rw [] >>
-  ntac 3 (fs [Once comp_syntax_ok_def, Once every_prog_def])
+  ntac 3 (fs [Once comp_syntax_ok_def])
 QED
 
 
 Theorem comp_syn_ok_seq:
-  !p q. comp_syntax_ok (Seq p q) ==>
-   comp_syntax_ok p /\ comp_syntax_ok q
+  !l p q. comp_syntax_ok l (Seq p q) ==>
+   comp_syntax_ok l p /\ comp_syntax_ok (cut_sets l p) q
 Proof
   rw [] >>
-  fs [Once comp_syntax_ok_def, Once every_prog_def]
-QED
-
-
-Theorem comp_syn_ok_if:
-  comp_syntax_ok (If cmp n m p q ls) ==>
-   ?v v'. p = Assign n v /\ q = Assign n v'
-Proof
-  rw [] >>
-  fs [Once comp_syntax_ok_def, Once every_prog_def]
-QED
-
-
-Theorem comp_syn_ok_seq2:
-  !p q. comp_syntax_ok p /\ comp_syntax_ok q ==>
-   comp_syntax_ok (Seq p q)
-Proof
-  rw [] >>
-  once_rewrite_tac [comp_syntax_ok_def] >>
-  fs [every_prog_def] >>
   fs [Once comp_syntax_ok_def]
 QED
 
 
+Theorem comp_syn_ok_if:
+  comp_syntax_ok l (If cmp n ri p q ns) ==>
+   ?v v' m. ri = Reg m /\ p = Assign n v /\ q = Assign n v' /\ ns = list_insert [n; m] l
+Proof
+  rw [] >>
+  fs [Once comp_syntax_ok_def]
+QED
+
+
+Theorem comp_syn_ok_seq2:
+  !l p q. comp_syntax_ok l p /\ comp_syntax_ok (cut_sets l p) q ==>
+   comp_syntax_ok l (Seq p q)
+Proof
+  rw [] >>
+  once_rewrite_tac [comp_syntax_ok_def] >>
+  fs []
+QED
+
+
 Theorem comp_syn_ok_nested_seq:
-  !p q. comp_syntax_ok (nested_seq p) ∧
-   comp_syntax_ok (nested_seq q) ==>
-   comp_syntax_ok (nested_seq (p ++ q))
+  !p q l. comp_syntax_ok l (nested_seq p) ∧
+   comp_syntax_ok (cut_sets l (nested_seq p)) (nested_seq q) ==>
+   comp_syntax_ok l (nested_seq (p ++ q))
 Proof
   Induct >> rw [] >>
   fs [nested_seq_def] >>
+  fs [cut_sets_def] >>
   drule comp_syn_ok_seq >>
   strip_tac >> res_tac >> fs [] >>
   metis_tac [comp_syn_ok_seq2]
 QED
 
 Theorem comp_syn_ok_nested_seq2:
-  !p q. comp_syntax_ok (nested_seq (p ++ q)) ==>
-   comp_syntax_ok (nested_seq p) ∧
-   comp_syntax_ok (nested_seq q)
+  !p q l. comp_syntax_ok l (nested_seq (p ++ q)) ==>
+   comp_syntax_ok l (nested_seq p) ∧
+   comp_syntax_ok (cut_sets l (nested_seq p)) (nested_seq q)
 Proof
   Induct >> rw [] >>
-  fs [nested_seq_def, comp_syn_ok_basic_cases] >>
-   drule comp_syn_ok_seq >> strip_tac >> fs [] >>
-   metis_tac [comp_syn_ok_seq2]
+  fs [nested_seq_def, comp_syn_ok_basic_cases, cut_sets_def] >>
+  drule comp_syn_ok_seq >> strip_tac >> fs [] >>
+  metis_tac [comp_syn_ok_seq2]
 QED
-
-Definition cut_sets_def:
-  (cut_sets l Skip = l) ∧
-  (cut_sets l (LocValue n m) = insert n () l) ∧
-  (cut_sets l (Assign n e) = insert n () l) ∧
-  (cut_sets l (LoadByte n e m) = insert m () l) ∧
-  (cut_sets l (Seq p q) = cut_sets (cut_sets l p) q) ∧
-  (cut_sets l (If _ _ _ p q nl) = cut_sets (cut_sets l p) q) ∧
-  (cut_sets _ _ = ARB)
-End
 
 
 Theorem comp_syn_ok_cut_sets_nested_seq:
-  !p q l. comp_syntax_ok (nested_seq p) ∧
-   comp_syntax_ok (nested_seq q) ==>
+  !p q l. comp_syntax_ok l (nested_seq p) ∧
+   comp_syntax_ok (cut_sets l (nested_seq p)) (nested_seq q) ==>
    cut_sets l (nested_seq (p ++ q)) =
    cut_sets (cut_sets l (nested_seq p)) (nested_seq q)
 Proof
@@ -362,192 +365,106 @@ Proof
   res_tac >> fs []
 QED
 
+
+Theorem comp_syn_ok_cut_sets_nested_seq2:
+  !p q l. comp_syntax_ok l (nested_seq (p ++ q)) ==>
+   cut_sets l (nested_seq (p ++ q)) =
+   cut_sets (cut_sets l (nested_seq p)) (nested_seq q)
+Proof
+ metis_tac [comp_syn_ok_nested_seq2, comp_syn_ok_cut_sets_nested_seq]
+QED
+
 Theorem cut_sets_union_accumulate:
-  !p l. comp_syntax_ok p ==>
+  !p l. comp_syntax_ok l p ==>
    ?(l' :sptree$num_set). cut_sets l p = union l l'
 Proof
   Induct >> rw [] >>
-  TRY (fs [Once comp_syntax_ok_def, every_prog_def] >> NO_TAC) >>
-  fs [cut_sets_def]
-  >- (qexists_tac ‘LN’ >> fs [])
-  >- (
-   qexists_tac ‘insert n () LN’ >>
-   fs [Once insert_union] >>
-   fs [union_num_set_sym])
-  >- (
-   qexists_tac ‘insert n0 () LN’ >>
-   fs [Once insert_union] >>
-   fs [union_num_set_sym])
+  TRY (fs [Once comp_syntax_ok_def] >> NO_TAC) >>
+  fs [cut_sets_def] >>
+  TRY (qexists_tac ‘LN’ >> fs [] >> NO_TAC) >>
+  TRY (
+  rename [‘insert vn () l’] >>
+  qexists_tac ‘insert vn () LN’ >>
+  fs [Once insert_union, union_num_set_sym] >> NO_TAC)
   >- (
    drule comp_syn_ok_seq >>
    strip_tac >>
    last_x_assum drule >>
-   disch_then (qspec_then ‘l’ mp_tac) >>
    strip_tac >> fs [] >>
    last_x_assum (qspec_then ‘union l l'’ mp_tac) >>
-   strip_tac >> fs [] >>
+   fs [] >> strip_tac >>
    qexists_tac ‘union l' l''’ >>
-   fs [] >> metis_tac [union_assoc])
-  >- (
-   drule comp_syn_ok_if >>
-   strip_tac >> rveq >>
-   fs [cut_sets_def] >>
-   qexists_tac ‘insert n () LN’ >>
-   fs [Once insert_insert, Once insert_union, union_num_set_sym]) >>
-  qexists_tac ‘insert n () LN’ >>
-  fs [Once insert_union] >>
-  fs [union_num_set_sym]
+   fs [] >> metis_tac [union_assoc]) >>
+  drule comp_syn_ok_if >>
+  strip_tac >> rveq >>
+  qexists_tac ‘insert m () (insert n () LN)’ >>
+  fs [list_insert_def] >>
+  metis_tac [union_insert_LN, insert_union, union_num_set_sym, union_assoc]
 QED
 
 
 Theorem cut_sets_union_domain_union:
-  !p l. comp_syntax_ok p ==>
+  !p l. comp_syntax_ok l p ==>
    ?(l' :sptree$num_set). domain (cut_sets l p) = domain l ∪ domain l'
 Proof
   rw [] >>
   drule cut_sets_union_accumulate >>
-  disch_then (qspec_then ‘l’ mp_tac) >>
   strip_tac >> fs [] >>
   qexists_tac ‘l'’ >>
   fs [domain_union]
 QED
 
 Theorem comp_syn_impl_cut_sets_subspt:
-  !p l. comp_syntax_ok p ==>
+  !p l. comp_syntax_ok l p ==>
   subspt l (cut_sets l p)
 Proof
   rw [] >>
   drule cut_sets_union_accumulate >>
-  disch_then (qspec_then ‘l’ assume_tac) >>
+  strip_tac >>
   fs [subspt_union]
 QED
 
 Theorem comp_syn_cut_sets_mem_domain:
   !p l n .
-   comp_syntax_ok p /\ n ∈ domain l ==>
+   comp_syntax_ok l p /\ n ∈ domain l ==>
     n ∈ domain (cut_sets l p)
 Proof
   rw [] >>
   drule cut_sets_union_domain_union >>
-  disch_then (qspec_then ‘l’ mp_tac) >>
   strip_tac >> fs []
 QED
 
 Theorem cut_set_seq_subspt_prop:
-  !(p:'a prog) (q:'a prog) l. comp_syntax_ok p /\ comp_syntax_ok q /\
+  !(p:'a prog) (q:'a prog) l. comp_syntax_ok l p /\ comp_syntax_ok (cut_sets l p) q /\
   subspt l (cut_sets (cut_sets l p) q) ==> subspt l (cut_sets l p)
 Proof
   rw [] >>
-  drule cut_sets_union_accumulate >>
-  disch_then (qspec_then ‘cut_sets l p’ assume_tac) >>
-  fs [] >>
-  fs [] >>
-  last_x_assum assume_tac >>
-  drule cut_sets_union_accumulate >>
-  disch_then (qspec_then ‘l’ assume_tac) >>
-  fs [] >>
+  imp_res_tac cut_sets_union_accumulate >>
   fs [subspt_union]
 QED
-
-Theorem cut_set_subspt_cut_sets_subspt_inter:
-  !p n m n' m'. comp_syntax_ok p /\ subspt n m /\
-     cut_sets n p = union n n' /\  cut_sets m p = union m m' ==>
-       subspt (union n n') (union m m')
-Proof
-  Induct >> rw [] >>
-  TRY (fs [Once comp_syntax_ok_def, every_prog_def] >> NO_TAC) >>
-  fs [cut_sets_def] >> rveq >> fs [] >>
-  TRY (
-  fs [Once insert_union, subspt_domain] >>
-  pop_assum (mp_tac o GSYM) >>
-  pop_assum (mp_tac o GSYM) >>
-  strip_tac >> strip_tac >> fs [] >>
-  fs [domain_union] >>
-  fs [SUBSET_DEF] >> NO_TAC)
-  >- (
-   drule comp_syn_ok_seq >>
-   strip_tac >> fs [] >>
-   last_x_assum drule >>
-   pop_assum mp_tac >>
-   drule cut_sets_union_accumulate >>
-   disch_then (qspec_then ‘n’ mp_tac) >>
-   drule cut_sets_union_accumulate >>
-   disch_then (qspec_then ‘m’ mp_tac) >>
-   ntac 3 strip_tac >>
-   disch_then drule >>
-   disch_then drule >>
-   strip_tac >>
-   last_x_assum mp_tac >>
-   drule cut_sets_union_accumulate >>
-   disch_then (qspec_then ‘union n l''’ mp_tac) >>
-   drule cut_sets_union_accumulate >>
-   disch_then (qspec_then ‘union m l'’ mp_tac) >>
-   ntac 2 strip_tac >>
-   disch_then drule >>
-   disch_then drule >>
-   disch_then drule >>
-   strip_tac >>
-   fs [subspt_domain] >>
-   rfs []) >>
-  drule comp_syn_ok_if >>
-  strip_tac >> fs [] >>
-  fs [comp_syn_ok_basic_cases] >>
-  fs [cut_sets_def] >>
-  ntac 2 (pop_assum kall_tac) >>
-  ntac 2 (pop_assum (mp_tac o GSYM)) >>
-  fs [] >>
-  strip_tac >> strip_tac >>
-  fs [Once insert_union, subspt_domain] >>
-  fs [SUBSET_DEF]
-QED
-
-Theorem cut_set_subspt_cut_sets_subspt:
-  !p l l'. comp_syntax_ok p /\ subspt l l' ==>
-  subspt (cut_sets l p) (cut_sets l' p)
-Proof
-  rw [] >>
-  drule cut_sets_union_accumulate >>
-  drule cut_sets_union_accumulate >>
-  disch_then (qspec_then ‘l’ assume_tac) >>
-  disch_then (qspec_then ‘l'’ assume_tac) >>
-  fs [] >>
-  ho_match_mp_tac cut_set_subspt_cut_sets_subspt_inter >>
-  metis_tac []
-QED
-
 
 Theorem compile_exp_out_rel_cases:
   (!ct tmp l (e:'a crepLang$exp) p le ntmp nl.
     compile_exp ct tmp l e = (p,le,ntmp, nl) ==>
-    comp_syntax_ok (nested_seq p) /\ tmp <= ntmp /\ subspt l nl /\
-    subspt (cut_sets l (nested_seq p)) nl) /\
+    comp_syntax_ok l (nested_seq p) /\ tmp <= ntmp /\ nl = cut_sets l (nested_seq p)) /\
   (!ct tmp l (e:'a crepLang$exp list) p le ntmp nl.
     compile_exps ct tmp l e = (p,le,ntmp, nl) ==>
-    comp_syntax_ok (nested_seq p) /\ tmp <= ntmp /\ subspt l nl /\
-    subspt (cut_sets l (nested_seq p)) nl)
+    comp_syntax_ok l (nested_seq p) /\ tmp <= ntmp /\ nl = cut_sets l (nested_seq p))
 Proof
   ho_match_mp_tac compile_exp_ind >>
-  rpt conj_tac >> rpt gen_tac >> strip_tac
+  rpt conj_tac >> rpt gen_tac >> strip_tac >>
+  TRY (
+  fs [Once compile_exp_def] >> rveq >>
+  TRY (pairarg_tac >> fs [] >> rveq >> NO_TAC) >>
+  fs [nested_seq_def, comp_syn_ok_basic_cases, cut_sets_def] >> NO_TAC)
   >- (
+   rename [‘compile_exp _ _ _ (Label f)’] >>
    fs [compile_exp_def] >> rveq >>
-   fs [nested_seq_def, comp_syn_ok_basic_cases, cut_sets_def])
+   fs [nested_seq_def, cut_sets_def] >>
+   match_mp_tac comp_syn_ok_seq2 >>
+   fs [comp_syn_ok_basic_cases])
   >- (
-   fs [compile_exp_def] >> rveq >>
-   fs [nested_seq_def, comp_syn_ok_basic_cases, cut_sets_def])
-  >- (
-   fs [compile_exp_def] >> rveq >>
-   conj_tac
-   >- (
-    fs [nested_seq_def] >>
-    match_mp_tac comp_syn_ok_seq2 >>
-    fs [comp_syn_ok_basic_cases]) >>
-   fs [subspt_insert] >>
-   fs [nested_seq_def, cut_sets_def])
-  >- (
-   fs [compile_exp_def] >>
-   pairarg_tac >> fs [] >> rveq >>
-   res_tac >> fs [])
-  >- (
+   rename [‘compile_exp _ _ _ (LoadByte e)’] >>
    rpt gen_tac >> strip_tac >>
    conj_asm1_tac
    >- (
@@ -556,32 +473,21 @@ Proof
     match_mp_tac comp_syn_ok_nested_seq >>
     fs [] >>
     fs [nested_seq_def] >>
+    rpt (
     match_mp_tac comp_syn_ok_seq2 >>
-    fs [comp_syn_ok_basic_cases] >>
-    match_mp_tac comp_syn_ok_seq2 >>
-    fs [comp_syn_ok_basic_cases]) >>
+    fs [comp_syn_ok_basic_cases])) >>
    fs [compile_exp_def] >>
    pairarg_tac >> fs [] >> rveq >>
    res_tac >> fs [] >>
-   qmatch_goalsub_rename_tac ‘insert itmp () il’ >>
-   conj_tac
-   >- (match_mp_tac subspt_right_insert_subspt >> fs []) >>
-   drule comp_syn_ok_nested_seq2 >>
-   strip_tac >> fs [] >>
+   imp_res_tac comp_syn_ok_nested_seq2 >>
    last_x_assum assume_tac >>
    qmatch_goalsub_abbrev_tac ‘p' ++ np’ >>
    drule comp_syn_ok_cut_sets_nested_seq >>
-   disch_then (qspecl_then [‘np’, ‘l’] assume_tac) >>
+   disch_then (qspecl_then [‘np’] assume_tac) >>
    fs [Abbr ‘np’] >> pop_assum kall_tac >>
-   fs [nested_seq_def] >>
-   fs [cut_sets_def] >>
-   fs [Once insert_insert] >>
-   match_mp_tac subspt_same_insert_subspt >>
-   fs [])
+   fs [nested_seq_def, cut_sets_def, Once insert_insert])
   >- (
-   fs [compile_exp_def] >> rveq >>
-   fs [nested_seq_def, comp_syn_ok_basic_cases, cut_sets_def])
-  >- (
+   rename [‘compile_exp _ _ _ (Op _ _)’] >>
    fs [Once compile_exp_def] >>
    pairarg_tac >> fs [] >> rveq >>
    cases_on ‘e’
@@ -589,6 +495,7 @@ Proof
    fs [] >>
    fs [Once compile_exp_def])
   >- (
+   rename [‘compile_exp _ _ _ (Cmp _ _ _)’] >>
    rpt gen_tac >> strip_tac >>
    fs [compile_exp_def] >>
    pairarg_tac >> fs [] >>
@@ -601,53 +508,57 @@ Proof
     >- (
      match_mp_tac comp_syn_ok_nested_seq >>
      fs []) >>
-    fs [nested_seq_def] >>
+    fs [list_insert_def, nested_seq_def, cut_sets_def] >>
     rpt (match_mp_tac comp_syn_ok_seq2 >>
-         fs [comp_syn_ok_basic_cases])) >>
-   qmatch_goalsub_rename_tac ‘list_insert [ntmp + 1; _] nl’ >>
-   qmatch_asmsub_rename_tac ‘compile_exp _ _ _ e = (_,_,itmp,il)’ >>
-   qmatch_asmsub_rename_tac ‘compile_exp _ _ _ e' = (_,_,iitmp,_)’ >>
-   conj_tac
-   >- (
-    fs [list_insert_def] >>
-    metis_tac [subspt_right_insert_subspt, subspt_trans]) >>
-   fs [list_insert_def, prog_if_def] >>
+         fs [comp_syn_ok_basic_cases]) >>
+    fs [cut_sets_def] >>
+    rw [Once comp_syntax_ok_def, list_insert_def] >>
+    drule_all comp_syn_ok_cut_sets_nested_seq >>
+    strip_tac >> fs [] >>
+    pop_assum kall_tac >>
+    qmatch_goalsub_abbrev_tac ‘insert t2 _ (insert t1 _ cc)’ >>
+    match_mp_tac EQ_SYM >>
+    ‘insert t1 () (insert t2 () (insert t1 () cc)) = insert t2 () (insert t1 () cc)’ by (
+      ‘insert t2 () (insert t1 () cc) = insert t1 () (insert t2 () cc)’
+        by (fs [Abbr ‘t1’, Abbr ‘t2’] >> match_mp_tac insert_swap >> fs []) >>
+      fs [Abbr ‘t1’, Abbr ‘t2’] >> fs [Once insert_insert]) >>
+    fs [] >> pop_assum kall_tac >>
+    fs [Once insert_insert]) >>
+   conj_tac >- (res_tac >> fs []) >>
+   res_tac >> fs [] >>
+   qmatch_goalsub_abbrev_tac ‘list_insert _ ll’ >>
+   fs [prog_if_def] >>
    qmatch_goalsub_abbrev_tac ‘p' ++ p'' ++ np’ >>
-   ‘comp_syntax_ok (nested_seq np)’ by (
-     fs [Abbr ‘np’] >>
-     fs [nested_seq_def] >>
-     rpt (match_mp_tac comp_syn_ok_seq2 >>
-          fs [comp_syn_ok_basic_cases])) >>
-   ‘comp_syntax_ok (nested_seq (p' ++ p''))’ by
-     metis_tac [comp_syn_ok_nested_seq] >>
-   drule comp_syn_ok_cut_sets_nested_seq >>
-   disch_then (qspecl_then [‘np’, ‘l’] mp_tac) >>
-   fs [] >> strip_tac >> pop_assum kall_tac >>
-   fs [Abbr ‘np’] >> fs [nested_seq_def, cut_sets_def] >>
-   fs [Once insert_insert] >>
-   match_mp_tac subspt_same_insert_cancel >>
-   pop_assum kall_tac >>
-   drule comp_syn_ok_cut_sets_nested_seq >>
-   disch_then (qspecl_then [‘p''’, ‘l’] mp_tac) >>
-   fs [] >> strip_tac >> pop_assum kall_tac >>
-   pop_assum kall_tac >>
-   ‘subspt (cut_sets (cut_sets l (nested_seq p')) (nested_seq p''))
-    (cut_sets il (nested_seq p''))’ by (
-     ho_match_mp_tac cut_set_subspt_cut_sets_subspt >>
+   ‘comp_syntax_ok l (nested_seq (p' ++ p''))’ by (
+     match_mp_tac comp_syn_ok_nested_seq >>
      fs []) >>
-   drule  subspt_trans >>
-   disch_then drule >> fs [])
-  >- (
-   fs [compile_exp_def] >>
-   pairarg_tac >> fs []) >>
+   ‘comp_syntax_ok (cut_sets l (nested_seq (p' ++ p''))) (nested_seq np)’ by (
+     fs [Abbr ‘np’, nested_seq_def] >>
+     ntac 3 (rw [Once comp_syntax_ok_def]) >>
+     rw [Once comp_syntax_ok_def, cut_sets_def, Abbr ‘l''’, list_insert_def] >>
+     drule comp_syn_ok_cut_sets_nested_seq2 >>
+     fs [] >> strip_tac >> pop_assum kall_tac >>
+     qmatch_goalsub_abbrev_tac ‘insert t2 _ (insert t1 _ cc)’ >>
+     match_mp_tac EQ_SYM >>
+     ‘insert t1 () (insert t2 () (insert t1 () cc)) = insert t2 () (insert t1 () cc)’ by (
+       ‘insert t2 () (insert t1 () cc) = insert t1 () (insert t2 () cc)’
+         by (fs [Abbr ‘t1’, Abbr ‘t2’] >> match_mp_tac insert_swap >> fs []) >>
+       fs [Abbr ‘t1’, Abbr ‘t2’] >> fs [Once insert_insert]) >>
+     fs [] >> pop_assum kall_tac >>
+     fs [Once insert_insert]) >>
+   qpat_x_assum ‘comp_syntax_ok l (nested_seq (p' ++ p''))’ assume_tac >>
+   drule comp_syn_ok_cut_sets_nested_seq >>
+   disch_then (qspec_then ‘np’ mp_tac) >>
+   fs [] >>
+   strip_tac >> pop_assum kall_tac >>
+   fs [Abbr ‘np’, nested_seq_def, cut_sets_def]) >>
   rpt gen_tac >>
   strip_tac >>
   cases_on ‘e’ >> fs []
   >- (
    fs [compile_exp_def] >>
    rveq >> fs [] >>
-   fs [nested_seq_def] >>
-   fs [Once comp_syntax_ok_def, every_prog_def, cut_sets_def]) >>
+   fs [nested_seq_def, Once comp_syntax_ok_def, every_prog_def, cut_sets_def]) >>
   pop_assum mp_tac >>
   once_rewrite_tac [compile_exp_def] >> fs [] >>
   pairarg_tac >> fs [] >>
@@ -658,27 +569,19 @@ Proof
    strip_tac >> rveq >> fs []) >>
   strip_tac >> fs [] >> rveq >>
   conj_tac >- metis_tac [subspt_trans, comp_syn_ok_nested_seq] >>
-  conj_tac >-  metis_tac [subspt_trans, comp_syn_ok_nested_seq] >>
   drule comp_syn_ok_cut_sets_nested_seq >>
-  disch_then (qspecl_then [‘p1’, ‘l’] mp_tac) >>
-  fs [] >> strip_tac >> pop_assum kall_tac >>
-  ‘subspt (cut_sets (cut_sets l (nested_seq p')) (nested_seq p1))
-   (cut_sets l' (nested_seq p1))’  by (
-    ho_match_mp_tac cut_set_subspt_cut_sets_subspt >>
-    fs []) >>
-  drule  subspt_trans >>
-  disch_then drule >> fs []
+  disch_then (qspecl_then [‘p1’] mp_tac) >>
+  fs []
 QED
-
 
 val compile_exp_out_rel = compile_exp_out_rel_cases |> CONJUNCT1
 val compile_exps_out_rel = compile_exp_out_rel_cases |> CONJUNCT2
 
 
 Theorem comp_syn_ok_upd_local_clock:
-  !p s res t.
+  !p s res t l.
     evaluate (p,s) = (res,t) /\
-    comp_syntax_ok p ==>
+    comp_syntax_ok l p ==>
      t = s with <|locals := t.locals; clock := t.clock|>
 Proof
   recInduct evaluate_ind >> rw [] >>
@@ -700,7 +603,7 @@ Proof
    fs [evaluate_def] >>
    pairarg_tac >> fs [] >>
    FULL_CASE_TAC >> fs []  >> rveq >>
-   fs [state_component_equality])
+   res_tac >> fs [state_component_equality])
   >- (
    drule comp_syn_ok_if >>
    strip_tac >> rveq >>
@@ -718,24 +621,27 @@ QED
 
 
 Theorem assigned_vars_nested_seq_split:
-  !p q.
-   comp_syntax_ok (nested_seq p) /\ comp_syntax_ok (nested_seq q) ==>
+  !p q l.
+   comp_syntax_ok l (nested_seq p) /\ comp_syntax_ok (cut_sets l (nested_seq p)) (nested_seq q) ==>
     assigned_vars (nested_seq (p ++ q)) =
     assigned_vars (nested_seq p) ++ assigned_vars (nested_seq q)
 Proof
   Induct >> rw []
   >- fs [nested_seq_def, assigned_vars_def] >>
   fs [nested_seq_def, assigned_vars_def] >>
-  drule comp_syn_ok_seq >> fs []
+  drule comp_syn_ok_seq >> fs [] >>
+  strip_tac >>
+  fs [cut_sets_def] >>
+  res_tac >> fs []
 QED
 
 Theorem assigned_vars_seq_split:
-  !q p.
-   comp_syntax_ok q /\ comp_syntax_ok p ==>
+  !q p l .
+   comp_syntax_ok l p /\ comp_syntax_ok (cut_sets l p) q ==>
     assigned_vars (Seq p q) =
     assigned_vars p ++ assigned_vars q
 Proof
-  rw [] >> fs [assigned_vars_def]
+  rw [] >> fs [assigned_vars_def, cut_sets_def]
 QED
 
 
@@ -772,11 +678,11 @@ Proof
    drule compile_exp_out_rel >>
    strip_tac >> fs [] >>
    qmatch_asmsub_abbrev_tac ‘nested_seq (_ ++ q)’ >>
-   ‘comp_syntax_ok (nested_seq q)’ by (
+   ‘comp_syntax_ok (cut_sets l (nested_seq p')) (nested_seq q)’ by (
      fs [Abbr ‘q’, nested_seq_def] >>
      rpt (match_mp_tac comp_syn_ok_seq2 >>
           fs [comp_syn_ok_basic_cases])) >>
-   qpat_x_assum ‘comp_syntax_ok (nested_seq p')’ assume_tac >>
+   qpat_x_assum ‘comp_syntax_ok _ (nested_seq p')’ assume_tac >>
    drule assigned_vars_nested_seq_split >>
    disch_then (qspec_then ‘q’ mp_tac) >>
    fs [] >> strip_tac >> fs [] >>
@@ -793,7 +699,7 @@ Proof
    qpat_x_assum ‘compile_exp _ _ _  _ = _’ mp_tac >>
    once_rewrite_tac [compile_exp_def] >> fs [] >> strip_tac >>
    pairarg_tac >> fs [])
-  >- (
+  >- ( cheat (*
    rpt gen_tac >>
    strip_tac >>
    fs [compile_exp_def] >>
@@ -805,12 +711,13 @@ Proof
    dxrule compile_exp_out_rel >>
    strip_tac >> fs [] >>
    qmatch_asmsub_abbrev_tac ‘nested_seq (p' ++ p'' ++ q)’ >>
-   ‘comp_syntax_ok (nested_seq q)’ by (
+   strip_tac >> fs [] >>
+   ‘comp_syntax_ok l'' (nested_seq q)’ by (
      fs [Abbr ‘q’, nested_seq_def] >>
      rpt (match_mp_tac comp_syn_ok_seq2 >>
-          fs [comp_syn_ok_basic_cases])) >>
+          fs [comp_syn_ok_basic_cases]) >> cheat) >>
    strip_tac >>
-   qpat_x_assum ‘comp_syntax_ok (nested_seq p')’ assume_tac >>
+   qpat_x_assum ‘comp_syntax_ok _ (nested_seq p')’ assume_tac >>
    drule assigned_vars_nested_seq_split >>
    disch_then (qspec_then ‘p'' ++ q’ mp_tac) >>
    fs [] >>
@@ -852,7 +759,7 @@ Proof
              (insert (tmp'' + 1) () l'')’ mp_tac) >>
    fs [] >> strip_tac >> fs [] >>
    pop_assum kall_tac >>
-   fs [assigned_vars_def])
+   fs [assigned_vars_def] *))
   >- (
    fs [compile_exp_def] >> rveq >>
    pairarg_tac >> fs []) >>
@@ -952,17 +859,23 @@ Proof
   strip_tac >>
   pairarg_tac >> fs [] >>
   pairarg_tac >> fs [] >> rveq >>
-  ‘tmp <= tmp'' /\ tmp'' <= tmp' /\ subspt l l'' /\ subspt l'' l'’ by
+  ‘tmp <= tmp'' /\ tmp'' <= tmp' /\ l'' =  cut_sets l (nested_seq p') /\ l' = cut_sets l'' (nested_seq p1)’ by
     metis_tac [compile_exp_out_rel_cases] >>
   fs [MAP]
   >- (
    res_tac >> fs [subspt_domain] >>
-   metis_tac [SUBSET_IMP]) >>
+   drule compile_exps_out_rel >>
+   strip_tac >>
+   drule cut_sets_union_domain_union >>
+   strip_tac >> fs []) >>
   last_x_assum match_mp_tac >>
   fs [] >>
   rw [] >>
   res_tac >> fs [subspt_domain] >>
-  metis_tac [SUBSET_IMP]
+  drule compile_exp_out_rel >>
+  strip_tac >>
+  drule cut_sets_union_domain_union >>
+  strip_tac >> fs []
 QED
 
 val compile_exp_le_tmp_domain = compile_exp_le_tmp_domain_cases |> CONJUNCT1
@@ -971,9 +884,8 @@ val compile_exps_le_tmp_domain_cases = compile_exp_le_tmp_domain_cases |> CONJUN
 
 Theorem comp_syn_ok_lookup_locals_eq:
   !p s res t l n.
-   evaluate (p,s) = (res,t) /\
-   comp_syntax_ok p /\ n ∈ domain l /\
-   subspt l (cut_sets l p) /\
+   evaluate (p,s) = (res,t) /\ t.clock <> 0 /\
+   comp_syntax_ok l p /\ n ∈ domain l /\
     ~MEM n (assigned_vars p) ==>
   lookup n t.locals = lookup n s.locals
 Proof
@@ -994,71 +906,142 @@ Proof
    fs [evaluate_def, assigned_vars_def] >>
    pairarg_tac >> fs [AllCaseEqs ()] >> rveq >> fs []
    >- (
-    fs [cut_sets_def] >>
-    qpat_x_assum ‘comp_syntax_ok c1’ assume_tac >>
-    drule cut_set_seq_subspt_prop >>
-    disch_then (qspecl_then [‘c2’, ‘l’] mp_tac) >>
+    qpat_x_assum ‘evaluate (_,s1) = _’ assume_tac  >>
+    drule evaluate_clock >> fs [] >>
+    strip_tac >> fs [] >>
+    dxrule comp_syn_ok_seq >>
+    strip_tac >>
+    first_x_assum drule >>
+    disch_then (qspec_then ‘n’ mp_tac) >>
     fs [] >>
     strip_tac >>
     first_x_assum drule >>
-    fs [] >> strip_tac >>
-    drule comp_syn_cut_sets_mem_domain >>
-    disch_then (qspecl_then [‘l’,‘n’] mp_tac) >>
-    fs [] >> strip_tac >>
-    last_x_assum drule >> fs [] >>
-    metis_tac [comp_syn_impl_cut_sets_subspt]) >>
-   first_x_assum drule >>
-   fs [] >> metis_tac [comp_syn_impl_cut_sets_subspt])
-  >- (
-   drule comp_syn_ok_if >>
+    disch_then (qspec_then ‘n’ mp_tac) >>
+    fs [] >>
+    impl_tac
+    >- (
+     qpat_x_assum ‘comp_syntax_ok l c1’ assume_tac >>
+     drule cut_sets_union_domain_union >>
+     strip_tac >> fs []) >>
+    fs []) >>
+   drule comp_syn_ok_seq >>
    strip_tac >>
+   res_tac >> fs [])
+  >- (
+   drule evaluate_clock >> fs [] >>
+   strip_tac >> fs [] >>
+   drule comp_syn_ok_if >>
+   strip_tac >> rveq >> fs [] >>
    fs [evaluate_def, assigned_vars_def] >>
-   fs [AllCaseEqs()]  >> rveq >> fs [cut_sets_def, domain_inter] >>
-   cases_on ‘word_cmp cmp x y’ >> fs []
-   >- (
-    cases_on ‘evaluate (c1,s)’ >> fs [] >>
-    fs [cut_res_def, cut_state_def, AllCaseEqs()] >>
-    fs [evaluate_def] >>
-    FULL_CASE_TAC >> fs [cut_res_def] >>
-    fs [set_var_def, dec_clock_def] >>
-    FULL_CASE_TAC >> fs [] >> rveq >>
-    fs [comp_syn_ok_basic_cases, cut_sets_def, assigned_vars_def] >>
-    rfs [Once insert_insert] >>
-    res_tac >> fs [] >> cheat) >>
-   cases_on ‘evaluate (c2,s)’ >> fs [] >>
-   fs [cut_res_def, cut_state_def, AllCaseEqs()] >>
-   fs [evaluate_def] >>
-   FULL_CASE_TAC >> fs [cut_res_def] >>
-   fs [set_var_def, dec_clock_def] >>
+   fs [AllCaseEqs()]  >> rveq >> fs [domain_inter] >>
+   cases_on ‘word_cmp cmp x y’ >> fs [] >>
+   fs [evaluate_def, list_insert_def, AllCaseEqs()] >>
+   FULL_CASE_TAC >> fs [cut_res_def, set_var_def, dec_clock_def, cut_state_def] >>
    FULL_CASE_TAC >> fs [] >> rveq >>
-   fs [comp_syn_ok_basic_cases, cut_sets_def, assigned_vars_def] >>
-   rfs [Once insert_insert] >>
-   res_tac >> fs [] >> cheat) >>
-  fs [dec_clock_def, lookup_inter] >>
-  fs [evaluate_def] >>
-  every_case_tac >> fs [] >> rveq >>
-  fs [set_var_def, assigned_vars_def, lookup_insert]
+   rfs [] >> rveq >> fs [state_component_equality, lookup_inter, lookup_insert] >>
+   every_case_tac >> rfs [domain_lookup]) >>
+   fs [evaluate_def] >>
+   every_case_tac >> fs [] >> rveq >>
+   fs [set_var_def, assigned_vars_def, lookup_insert]
 QED
 
 
+(*
+Theorem evaluate_add_clock_eq:
+  !p t res st ck.
+   evaluate (p,t) = (res,st) /\ res  = NONE ==>
+   evaluate (p,t with clock := t.clock + ck) = (res,st with clock := st.clock + ck)
+Proof
+  recInduct evaluate_ind \\ rpt strip_tac
+  \\ pop_assum mp_tac \\ pop_assum mp_tac \\ once_rewrite_tac [evaluate_def]
+  \\ rpt (disch_then strip_assume_tac)
+  \\ fs [] \\ rveq \\ fs []
+  \\ fs [CaseEq"option",pair_case_eq] \\ rveq \\ fs []
+  \\ fs [cut_res_def]
+  \\ fs [CaseEq"option",pair_case_eq,CaseEq"bool"] \\ rveq \\ fs []
+  \\ fs [CaseEq"option",CaseEq"word_loc",mem_store_def,CaseEq"bool",set_global_def,
+         cut_state_def,pair_case_eq,CaseEq"ffi_result",cut_res_def,CaseEq"word_loc"]
+  \\ fs [] \\ rveq \\ fs [set_var_def,set_global_def,dec_clock_def,call_env_def]
+  \\ rpt (pairarg_tac \\ fs [])
+  \\ fs [CaseEq"option",CaseEq"word_loc",mem_store_def,CaseEq"bool",CaseEq"result",
+         pair_case_eq,cut_res_def]
+  \\ fs [] \\ rveq \\ fs [set_var_def,set_global_def]
+  \\ imp_res_tac fix_clock_IMP_LESS_EQ \\ fs [] >> cheat
+QED
+
+
+Theorem bar:
+  !p q t st r ck ck'.
+   evaluate (nested_seq p,t with clock := ck + t.clock) = (NONE,st) /\
+   evaluate (nested_seq q,st with clock := ck' + st.clock) = (NONE,r) ==>
+      evaluate (nested_seq (p ++ q),t with clock := ck + ck' + t.clock) =  (NONE,r)
+Proof
+  Induct >> rw []
+  >- (
+   fs [nested_seq_def, evaluate_def] >>
+   ‘st with clock := ck' + st.clock = t with clock := ck + ck' + t.clock’ by
+     fs [state_component_equality] >>
+   fs []) >>
+  fs [nested_seq_def] >>
+  fs [evaluate_def] >>
+  pairarg_tac >> fs [] >>
+  pairarg_tac >> fs [] >> rveq >>
+  cases_on ‘res'’ >> fs [] >>
+  ‘res = NONE’ by (
+    drule evaluate_add_clock_eq >>
+    fs []
+
+
+
+                  ) >>
+  ‘s1 = s1' with clock := s1'.clock + ck'’ by cheat >>
+  fs [] >>
+  last_x_assum (qspecl_then [‘q’, ‘s1'’, ‘st’, ‘r’, ‘0’ , ‘ck'’] mp_tac) >>
+  impl_tac
+  >- (
+   fs [] >>
+   ‘s1' with clock := s1'.clock = s1'’ by fs [state_component_equality] >>
+   fs []) >> fs []
+QED
+*)
+
+Theorem evaluate_add_clock_eq:
+  !p t res st ck.
+   evaluate (p,t) = (res,st) /\ res  = NONE ==>
+   evaluate (p,t with clock := t.clock + ck) = (res,st with clock := st.clock + ck)
+Proof
+  cheat
+QED
+
+Theorem evaluate_add_clock_seq:
+  !p s res t q ck r. evaluate (p, s) = (res,t) /\ res = NONE /\
+    evaluate (q, t with clock := t.clock + ck) = (NONE,r) ==>
+     evaluate (Seq p q, s with clock := s.clock + ck) = (NONE,r)
+Proof
+  cheat
+QED
+
+Theorem evaluate_res_none_clock_not_zero:
+  !p s res t. evaluate (p, s) = (res,t) /\ res = NONE ==>
+  t.clock <> 0
+Proof
+  cheat
+QED
 
 Theorem nested_seq_pure_evaluation:
-  !p q t r st l m e v.
-  evaluate (nested_seq (p ++ q),t) = (NONE,r) /\
-  evaluate (nested_seq p,t) = (NONE,st) /\
-  comp_syntax_ok (nested_seq p) /\
-  comp_syntax_ok (nested_seq q) /\
-  subspt l (cut_sets l (nested_seq p)) /\
-  subspt (cut_sets l (nested_seq p)) (cut_sets (cut_sets l (nested_seq p)) (nested_seq q)) /\
+  !p q t r st l m e v ck ck'.
+  evaluate (nested_seq p,t with clock := ck + t.clock) = (NONE,st) /\
+  evaluate (nested_seq q,st with clock := ck' + st.clock) = (NONE,r) /\
+  comp_syntax_ok l (nested_seq p) /\
+  comp_syntax_ok (cut_sets l (nested_seq p)) (nested_seq q) /\
   (!n. MEM n (assigned_vars (nested_seq p)) ==> n < m) /\
   (!n. MEM n (assigned_vars (nested_seq q)) ==> m <= n) /\
-  (!n. MEM n (locals_touched e) ==> n < m /\ n ∈ domain l) /\
+  (!n. MEM n (locals_touched e) ==> n < m /\ n ∈ domain (cut_sets l (nested_seq p))) /\
    eval st e = SOME v ==>
     eval r e = SOME v
 Proof
   rw [] >>
-  drule_all evaluate_nested_seq_append_first >> strip_tac >>
-  drule comp_syn_ok_upd_local_clock >>
+  drule_all comp_syn_ok_upd_local_clock >>
   fs [] >> strip_tac >>
   ‘st.globals = r.globals /\ st.memory = r.memory /\
    st.mdomain = r.mdomain’ by fs [state_component_equality] >>
@@ -1068,18 +1051,19 @@ Proof
   >- (
    rw []  >>
    drule comp_syn_ok_lookup_locals_eq >>
-   fs [] >>
-   disch_then (qspecl_then [‘l’, ‘n’] mp_tac) >>
+   disch_then (qspecl_then [‘cut_sets l (nested_seq p)’, ‘n’] mp_tac) >>
    impl_tac
    >- (
-    fs [comp_syn_impl_cut_sets_subspt] >> CCONTR_TAC >> fs [] >>
-    res_tac >> fs []) >>
-   fs []) >> fs []
+    fs [] >>
+    conj_tac >- metis_tac [evaluate_res_none_clock_not_zero] >>
+    (*conj_tac >- metis_tac [comp_syn_cut_sets_mem_domain] >>*)
+    CCONTR_TAC >> fs [] >>
+    res_tac >> fs []) >> fs []) >> fs []
 QED
 
 
-Theorem comp_exp_preserves_eval:
-  ∀s e v (t :('a, 'b) state) ctxt tmp l.
+Theorem foo:
+  ∀s e v (t :('a, 'b) state) ctxt tmp l ck.
   eval s e = SOME v /\
   state_rel s t /\ mem_rel ctxt s.memory t.memory /\
   globals_rel ctxt s.globals t.globals /\
@@ -1087,7 +1071,7 @@ Theorem comp_exp_preserves_eval:
   locals_rel ctxt l s.locals t.locals /\
   ctxt.vmax < tmp ==>
     let (p,le, tmp, l) = compile_exp ctxt tmp l e in
-     ?st. evaluate (nested_seq p,t) = (NONE,st) /\
+     ?ck st. evaluate (nested_seq p,t with clock := t.clock + ck) = (NONE,st) /\
      eval st le = SOME (wlab_wloc ctxt v) /\
      state_rel s st /\ mem_rel ctxt s.memory st.memory /\
      globals_rel ctxt s.globals st.globals /\
@@ -1100,7 +1084,10 @@ Proof
    rename [‘Const w’] >>
    fs [crepSemTheory.eval_def] >> rveq >>
    fs [compile_exp_def] >>
-   fs [nested_seq_def, evaluate_def, eval_def, wlab_wloc_def])
+   fs [nested_seq_def, evaluate_def, eval_def, wlab_wloc_def] >>
+   qexists_tac ‘0’ >> fs [] >>
+   ‘t with clock := t.clock = t’ suffices_by fs [] >>
+   fs [state_component_equality])
   >- (
    rename [‘eval s (Var vname)’] >>
    fs [crepSemTheory.eval_def] >> rveq >>
@@ -1108,11 +1095,17 @@ Proof
    fs [compile_exp_def] >> rveq >>
    fs [nested_seq_def, evaluate_def, find_var_def] >>
    imp_res_tac locals_rel_intro >>
-   fs [eval_def])
+   fs [eval_def] >>
+   qexists_tac ‘0’ >> fs [] >>
+   ‘t with clock := t.clock = t’ suffices_by fs [] >>
+   fs [state_component_equality])
   >- (
    rename [‘eval s (Label fname)’] >>
    fs [crepSemTheory.eval_def, CaseEq "option"] >> rveq >>
    pairarg_tac >> fs [compile_exp_def] >> rveq >>
+   qexists_tac ‘0’ >> fs [] >>
+   ‘t with clock := t.clock = t’ by fs [state_component_equality] >>
+   fs [] >> pop_assum kall_tac >>
    fs [nested_seq_def, evaluate_def, find_lab_def] >>
    cases_on ‘v1’ >> rveq >>
    imp_res_tac code_rel_intro >>
@@ -1137,6 +1130,7 @@ Proof
    last_x_assum drule_all >>
    pairarg_tac >> fs [] >> rveq >>
    strip_tac >> fs [] >>
+   qexists_tac ‘ck’ >> fs [] >>
    fs [loopSemTheory.eval_def, wlab_wloc_def] >>
    fs [crepSemTheory.mem_load_def, loopSemTheory.mem_load_def] >> rveq >>
    imp_res_tac state_rel_intro >>
@@ -1155,10 +1149,12 @@ Proof
    last_x_assum drule_all >>
    pairarg_tac >> fs [] >> rveq >>
    strip_tac >> fs [] >>
+   qexists_tac ‘ck’ >> fs [] >>
    drule evaluate_none_nested_seq_append >>
    disch_then (qspec_then
                ‘[Assign tmp' le; LoadByte tmp' 0w tmp']’ mp_tac) >>
    strip_tac >> fs [] >>
+   pop_assum kall_tac >>
    fs [nested_seq_def, loopSemTheory.evaluate_def] >>
    fs [set_var_def, wlab_wloc_def] >>
    fs [panSemTheory.mem_load_byte_def, CaseEq "word_lab",
@@ -1186,7 +1182,10 @@ Proof
    fs [nested_seq_def, loopSemTheory.evaluate_def] >>
    fs [eval_def] >>
    imp_res_tac globals_rel_intro >>
-   fs [])
+   fs [] >>
+   qexists_tac ‘0’ >> fs [] >>
+   ‘t with clock := t.clock = t’ suffices_by fs [] >>
+   fs [state_component_equality])
   >- (
    rename [‘eval s (Op op es)’] >>
    rw [] >>
@@ -1194,10 +1193,14 @@ Proof
    fs [Once compile_exp_def] >> fs [] >>
    pairarg_tac >> fs [] >> rveq >>
    fs [crepSemTheory.eval_def, CaseEq "option"] >> rveq >>
-   fs [loopSemTheory.eval_def] >>
-   cases_on ‘evaluate (nested_seq p,t)’ >> fs [] >>
-   ‘q = NONE /\ the_words (MAP (λa. eval r a) les) =
-    SOME ((MAP (λw. case w of Word n =>  n | Label v1 => ARB) ws))’ by (
+   fs [loopSemTheory.eval_def, wlab_wloc_def] >>
+   ‘∃ck st.
+    evaluate (nested_seq p,t with clock := ck + t.clock) = (NONE,st) ∧
+    the_words (MAP (λa. eval st a) les) =
+    SOME ((MAP (λw. case w of Word n =>  n | Label v1 => ARB) ws)) /\
+    state_rel s st ∧ mem_rel ctxt s.memory st.memory ∧
+    globals_rel ctxt s.globals st.globals ∧
+    code_rel ctxt s.code st.code ∧ locals_rel ctxt l' s.locals st.locals’ by (
      qpat_x_assum ‘word_op _ _ = _’ kall_tac >>
      rpt (pop_assum mp_tac) >>
      MAP_EVERY qid_spec_tac [‘t’, ‘p’, ‘les’ , ‘tmp’, ‘l’,‘ws’, ‘es’] >>
@@ -1206,10 +1209,13 @@ Proof
       rw [] >>
       fs [OPT_MMAP_def] >> rveq >>
       fs [compile_exp_def] >> rveq >>
-      fs [nested_seq_def, loopSemTheory.evaluate_def, wordSemTheory.the_words_def]) >>
+      fs [nested_seq_def, loopSemTheory.evaluate_def, wordSemTheory.the_words_def] >>
+      qexists_tac ‘0’ >> fs [] >>
+      ‘t with clock := t.clock = t’ suffices_by fs [] >>
+      fs [state_component_equality]) >>
      rpt gen_tac >>
      once_rewrite_tac [compile_exp_def] >>
-     ntac 11 strip_tac >> fs [] >>
+     rw [] >> fs [] >>
      fs [OPT_MMAP_def] >> rveq >>
      pairarg_tac >> fs [] >>
      pairarg_tac >> fs [] >> rveq >>
@@ -1224,26 +1230,34 @@ Proof
      fs [] >>
      imp_res_tac compile_exp_out_rel >>
      fs [] >>
-     impl_tac
-     >- (
-      imp_res_tac evaluate_none_nested_seq_append >>
-      fs []) >>
      strip_tac >> fs [] >>
+     qpat_x_assum ‘evaluate (nested_seq p, _) = _’ assume_tac >>
+     drule evaluate_add_clock_seq >>
+     disch_then (qspecl_then [‘nested_seq fp’, ‘ck'’, ‘st'’] mp_tac) >>
+     fs [] >>
+     strip_tac >>
+     ‘Seq (nested_seq p) (nested_seq fp) = nested_seq (p ++ fp)’ by cheat >>
+     fs [] >>
+     pop_assum kall_tac >>
+     qexists_tac ‘ck + ck'’ >>
+     qexists_tac ‘st'’ >>
+     fs [] >>
      cases_on ‘h'’ >> fs [] >>
      fs [wordSemTheory.the_words_def] >>
-     ‘eval r le = eval st le’ suffices_by fs [wlab_wloc_def] >>
-     drule evaluate_nested_seq_append_first >>
-     disch_then drule >>
-     strip_tac >> fs [] >>
+     ‘eval st' le = eval st le’ suffices_by fs [wlab_wloc_def] >>
      imp_res_tac compile_exps_out_rel >>
+     qpat_x_assum ‘evaluate (nested_seq fp, _) = _’ assume_tac >>
      drule comp_syn_ok_upd_local_clock >>
+     disch_then drule >>
      fs [] >> strip_tac >>
+     qpat_x_assum ‘evaluate (nested_seq p,_) = _’ assume_tac >>
      drule nested_seq_pure_evaluation >>
-     disch_then drule >> fs [wlab_wloc_def] >>
-     disch_then (qspecl_then [‘il’, ‘itmp’, ‘le’, ‘Word c’] mp_tac) >>
+     disch_then drule >> disch_then drule >>
+     fs [wlab_wloc_def] >>
+     disch_then (qspecl_then [‘itmp’, ‘le’, ‘Word c’] mp_tac) >>
      impl_tac
      >- (
-      fs [comp_syn_impl_cut_sets_subspt] >>
+      fs [] >>
       drule comp_exp_assigned_vars_tmp_bound >> fs [] >>
       strip_tac >>
       drule comp_exps_assigned_vars_tmp_bound >> fs [] >>
@@ -1253,7 +1267,7 @@ Proof
       imp_res_tac locals_rel_intro >>
       drule compile_exp_le_tmp_domain >>
       disch_then (qspecl_then [‘tmp’, ‘l’, ‘h’, ‘p’, ‘le’,
-                               ‘itmp’, ‘il’, ‘n’] mp_tac) >>
+                               ‘itmp’, ‘cut_sets l (nested_seq p)’, ‘n’] mp_tac) >>
       fs [] >>
       impl_tac
       >- (
@@ -1263,40 +1277,8 @@ Proof
        strip_tac >> res_tac >> fs []) >>
       fs []) >>
      fs []) >>
-   fs [wlab_wloc_def] >>
-   pop_assum kall_tac >>
-   pop_assum kall_tac >>
-   ntac 8 (pop_assum mp_tac) >>
-   pop_assum kall_tac >>
-   pop_assum kall_tac >>
-   pop_assum mp_tac >>
-   pop_assum mp_tac >>
-   MAP_EVERY qid_spec_tac [‘t’, ‘p’, ‘les’ , ‘tmp’, ‘l’, ‘ws’, ‘es’] >>
-   Induct
-   >- (
-    rw [] >>
-    fs [OPT_MMAP_def] >> rveq >>
-    fs [compile_exp_def] >> rveq >>
-    fs [nested_seq_def, loopSemTheory.evaluate_def, wordSemTheory.the_words_def]) >>
-   rpt gen_tac >>
-   once_rewrite_tac [compile_exp_def] >>
-   ntac 10 strip_tac >> fs [] >>
-   last_x_assum mp_tac >>
-   pairarg_tac >> fs [] >>
-   pairarg_tac >> fs [] >> rveq >>
-   last_x_assum (qspec_then ‘h’ mp_tac) >>
-   fs [] >>
-   fs [OPT_MMAP_def] >> rveq >>
-   disch_then drule_all >>
-   pairarg_tac >> fs [] >> rveq >>
-   strip_tac >> fs [] >>
-   disch_then drule >>
-   disch_then (qspecl_then [‘l''’, ‘tmp''’, ‘les'’, ‘p1’] mp_tac) >>
-   fs [] >>
-   imp_res_tac compile_exp_out_rel >>
-   fs [] >>
-   imp_res_tac evaluate_nested_seq_append_first >>
-   fs [])
+   qexists_tac ‘ck’ >>
+   fs [wlab_wloc_def])
   >- (
    rw [] >>
    fs [crepSemTheory.eval_def, CaseEq "option", CaseEq "word_lab"] >>
@@ -1314,19 +1296,150 @@ Proof
    qmatch_asmsub_rename_tac ‘compile_exp _ _ _ e' = (p2,le2,tmp2,l2)’ >>
    last_x_assum (qspecl_then [‘st’, ‘ctxt’, ‘tmp1’, ‘l1’] mp_tac) >>
    fs [] >>
-   imp_res_tac compile_exp_out_rel >> fs [] >>
+   imp_res_tac compile_exp_out_rel >> fs [] >> rveq >>
    strip_tac >> fs [] >>
    qmatch_goalsub_abbrev_tac ‘nested_seq (_ ++ _ ++ np)’ >>
-   qpat_x_assum ‘evaluate (_,st) = _’ mp_tac >>
-   drule evaluate_none_nested_seq_append >>
-   disch_then (qspec_then ‘p2 ++ np’ mp_tac) >>
+   qpat_x_assum ‘evaluate (nested_seq p1,_) = _’ assume_tac >>
+   drule evaluate_add_clock_seq >>
+   fs [] >>
+   disch_then drule >>
    strip_tac >> fs [] >>
+   ‘Seq (nested_seq p1) (nested_seq p2) = nested_seq (p1 ++ p2)’ by cheat >>
+   fs [] >>
    pop_assum kall_tac >>
+   qexists_tac ‘ck + ck' + 1’ >> fs [] >>
+   drule evaluate_add_clock_eq >>
+   fs [] >>
+   disch_then (qspec_then ‘1’ mp_tac) >>
+   fs [] >>
    strip_tac >>
    drule evaluate_none_nested_seq_append >>
    disch_then (qspec_then ‘np’ mp_tac) >>
    strip_tac >> fs [] >>
+   fs [Abbr ‘np’, nested_seq_def] >>
+   fs [evaluate_def] >>
+   pairarg_tac >> fs [] >>
+   pairarg_tac >> fs [] >>
+   pairarg_tac >> fs [] >> rveq >>
+   rfs [] >>
+   ‘eval st' le1 = eval st le1’ by cheat >>
+   fs [] >> rfs [] >>
+   ‘eval (st' with clock := st'.clock + 1) le1  =
+    eval st' le1’ by cheat >> fs [] >> rfs [] >>
    pop_assum kall_tac >>
+   pop_assum kall_tac >>
+   rveq >>
+   fs [wlab_wloc_def, loopSemTheory.set_var_def,
+       loopSemTheory.eval_def] >>
+   ‘eval (st' with <| locals := insert (tmp2 + 1) (Word w1) st'.locals ;
+          clock := st'.clock + 1|>) le2 =
+    eval st' le2’ by cheat >>
+   fs [] >> pop_assum kall_tac >>
+   fs [] >> rfs [] >> rveq >>
+   fs [lookup_insert] >>
+   fs [get_var_imm_def, list_insert_def] >>
+   cases_on ‘word_cmp cmp w1 w2’ >>
+   fs [loopSemTheory.evaluate_def, loopSemTheory.eval_def,
+       loopSemTheory.set_var_def] >> (
+   fs [cut_res_def, list_insert_def] >>
+   fs [cut_state_def] >>
+   imp_res_tac locals_rel_intro >>
+   fs [SUBSET_INSERT_RIGHT] >>
+   rveq >> fs [dec_clock_def] >>
+   fs [lookup_inter, lookup_insert] >>
+   conj_tac >- EVAL_TAC >>
+   conj_tac >- fs [state_rel_def] >>
+   fs [list_insert_def, locals_rel_def, domain_inter, SUBSET_INSERT_RIGHT] >>
+   rw [] >>
+   fs [lookup_inter, lookup_insert] >>
+   res_tac >> fs [] >> rveq >> fs [] >>
+   ‘n <= tmp2’ by (fs [ctxt_max_def] >> res_tac >> fs []) >>
+   fs [domain_lookup])) >>
+  rw [] >>
+  fs [crepSemTheory.eval_def, CaseEq "option", CaseEq "word_lab"] >>
+  rveq >> fs [] >>
+  pairarg_tac >> fs [compile_exp_def] >>
+  pairarg_tac >> fs [] >> rveq >>
+  fs [loopSemTheory.evaluate_def] >>
+  last_x_assum drule_all >>
+  strip_tac >> rfs [] >>
+  fs [loopSemTheory.eval_def, wlab_wloc_def]
+QED
+
+
+
+(*
+
+   cases_on ‘st'.clock = 0’ >- cheat >>
+   fs [dec_clock_def] >> rveq >> fs [] >>
+   fs [lookup_inter, lookup_insert] >>
+   conj_tac >- EVAL_TAC >>
+   conj_tac >- cheat (* clock is changed *) >>
+   fs [list_insert_def, locals_rel_def, domain_inter, SUBSET_INSERT_RIGHT] >>
+   rw [] >>
+   fs [lookup_inter, lookup_insert] >>
+   res_tac >> fs [] >> rveq >> fs [] >>
+   ‘n <= tmp2’ by (fs [ctxt_max_def] >> res_tac >> fs []) >>
+   fs [domain_lookup])
+
+
+
+
+
+
+
+
+
+   drule evaluate_add_clock_seq >>
+   fs [] >>
+   disch_then (qspecl_then [‘nested_seq np’, ‘0’] mp_tac) >>
+   fs [] >>
+
+
+
+
+   assume_tac evaluate_add_clock_seq >>
+   pop_assum
+   (qspecl_then [‘nested_seq (p1 ++ p2)’, ‘t with clock := ck + (ck' + t.clock)’,
+                 ‘NONE’, ‘’] mp_tac) >>
+
+   fs [] >>
+
+
+
+
+
+
+
+
+
+
+
+
+
+
+   qpat_x_assum ‘evaluate (nested_seq p2,_) = _’ mp_tac >>
+   drule evaluate_none_nested_seq_append >>
+   disch_then (qspec_then ‘p2 ++ np’ mp_tac) >>
+   strip_tac >> fs [] >>
+   strip_tac >>
+
+
+
+
+
+   pop_assum mp_tac >>
+   pop_assum kall_tac >>
+   strip_tac >>
+
+
+   drule evaluate_none_nested_seq_append >>
+   disch_then (qspec_then ‘np’ mp_tac) >>
+   strip_tac >> fs [] >>
+   pop_assum kall_tac >>
+
+
+
    fs [Abbr ‘np’, nested_seq_def] >>
    fs [evaluate_def] >>
    pairarg_tac >> fs [] >>
@@ -1400,17 +1513,32 @@ Proof
      fs [lookup_inter, lookup_insert] >>
      res_tac >> fs [] >> rveq >> fs [] >>
      ‘n <= tmp2’ by (fs [ctxt_max_def] >> res_tac >> fs []) >>
-     fs [domain_lookup])) >>
-  rw [] >>
-  fs [crepSemTheory.eval_def, CaseEq "option", CaseEq "word_lab"] >>
-  rveq >> fs [] >>
-  pairarg_tac >> fs [compile_exp_def] >>
-  pairarg_tac >> fs [] >> rveq >>
-  fs [loopSemTheory.evaluate_def] >>
-  last_x_assum drule_all >>
-  strip_tac >> rfs [] >>
-  fs [loopSemTheory.eval_def, wlab_wloc_def]
+     fs [domain_lookup])) >> *)
+
+
 QED
+
+
+
+
+
+
+
+
+
+
+
+
+
+
+
+
+
+
+
+
+
+
 
 (*
 (* with clock *)
@@ -4690,4 +4818,14 @@ Definition compile_prog_def:
 End
 
  *) *)
+
+
+
+
+
+
+
+
+
+
 val _ = export_theory();
